Add universe levels to Pi

theories/autosubst/AST.v
@@ -8,7 +8,7 @@ Module Core.
 Inductive term : Type :=
   | var : nat -> term
   | Sort : mode -> level -> term
-  | Pi : mode -> mode -> term -> term -> term
+  | Pi : level -> level -> mode -> mode -> term -> term -> term
   | lam : mode -> term -> term -> term
   | app : term -> term -> term
   | Erased : term -> term
@@ -28,16 +28,22 @@ exact (eq_trans (eq_trans eq_refl (ap (fun x => Sort x s1) H0))
          (ap (fun x => Sort t0 x) H1)).
 Qed.
 
-Lemma congr_Pi {s0 : mode} {s1 : mode} {s2 : term} {s3 : term} {t0 : mode}
-  {t1 : mode} {t2 : term} {t3 : term} (H0 : s0 = t0) (H1 : s1 = t1)
-  (H2 : s2 = t2) (H3 : s3 = t3) : Pi s0 s1 s2 s3 = Pi t0 t1 t2 t3.
+Lemma congr_Pi {s0 : level} {s1 : level} {s2 : mode} {s3 : mode} {s4 : term}
+  {s5 : term} {t0 : level} {t1 : level} {t2 : mode} {t3 : mode} {t4 : term}
+  {t5 : term} (H0 : s0 = t0) (H1 : s1 = t1) (H2 : s2 = t2) (H3 : s3 = t3)
+  (H4 : s4 = t4) (H5 : s5 = t5) : Pi s0 s1 s2 s3 s4 s5 = Pi t0 t1 t2 t3 t4 t5.
 Proof.
 exact (eq_trans
          (eq_trans
-            (eq_trans (eq_trans eq_refl (ap (fun x => Pi x s1 s2 s3) H0))
-               (ap (fun x => Pi t0 x s2 s3) H1))
-            (ap (fun x => Pi t0 t1 x s3) H2))
-         (ap (fun x => Pi t0 t1 t2 x) H3)).
+            (eq_trans
+               (eq_trans
+                  (eq_trans
+                     (eq_trans eq_refl (ap (fun x => Pi x s1 s2 s3 s4 s5) H0))
+                     (ap (fun x => Pi t0 x s2 s3 s4 s5) H1))
+                  (ap (fun x => Pi t0 t1 x s3 s4 s5) H2))
+               (ap (fun x => Pi t0 t1 t2 x s4 s5) H3))
+            (ap (fun x => Pi t0 t1 t2 t3 x s5) H4))
+         (ap (fun x => Pi t0 t1 t2 t3 t4 x) H5)).
 Qed.
 
 Lemma congr_lam {s0 : mode} {s1 : term} {s2 : term} {t0 : mode} {t1 : term}
@@ -135,8 +141,9 @@ Fixpoint ren_term (xi_term : nat -> nat) (s : term) {struct s} : term :=
   match s with
   | var s0 => var (xi_term s0)
   | Sort s0 s1 => Sort s0 s1
-  | Pi s0 s1 s2 s3 =>
-      Pi s0 s1 (ren_term xi_term s2) (ren_term (upRen_term_term xi_term) s3)
+  | Pi s0 s1 s2 s3 s4 s5 =>
+      Pi s0 s1 s2 s3 (ren_term xi_term s4)
+        (ren_term (upRen_term_term xi_term) s5)
   | lam s0 s1 s2 =>
       lam s0 (ren_term xi_term s1) (ren_term (upRen_term_term xi_term) s2)
   | app s0 s1 => app (ren_term xi_term s0) (ren_term xi_term s1)
@@ -167,9 +174,9 @@ term :=
   match s with
   | var s0 => sigma_term s0
   | Sort s0 s1 => Sort s0 s1
-  | Pi s0 s1 s2 s3 =>
-      Pi s0 s1 (subst_term sigma_term s2)
-        (subst_term (up_term_term sigma_term) s3)
+  | Pi s0 s1 s2 s3 s4 s5 =>
+      Pi s0 s1 s2 s3 (subst_term sigma_term s4)
+        (subst_term (up_term_term sigma_term) s5)
   | lam s0 s1 s2 =>
       lam s0 (subst_term sigma_term s1)
         (subst_term (up_term_term sigma_term) s2)
@@ -210,9 +217,10 @@ subst_term sigma_term s = s :=
   match s with
   | var s0 => Eq_term s0
   | Sort s0 s1 => congr_Sort (eq_refl s0) (eq_refl s1)
-  | Pi s0 s1 s2 s3 =>
-      congr_Pi (eq_refl s0) (eq_refl s1) (idSubst_term sigma_term Eq_term s2)
-        (idSubst_term (up_term_term sigma_term) (upId_term_term _ Eq_term) s3)
+  | Pi s0 s1 s2 s3 s4 s5 =>
+      congr_Pi (eq_refl s0) (eq_refl s1) (eq_refl s2) (eq_refl s3)
+        (idSubst_term sigma_term Eq_term s4)
+        (idSubst_term (up_term_term sigma_term) (upId_term_term _ Eq_term) s5)
   | lam s0 s1 s2 =>
       congr_lam (eq_refl s0) (idSubst_term sigma_term Eq_term s1)
         (idSubst_term (up_term_term sigma_term) (upId_term_term _ Eq_term) s2)
@@ -261,11 +269,11 @@ ren_term xi_term s = ren_term zeta_term s :=
   match s with
   | var s0 => ap (var) (Eq_term s0)
   | Sort s0 s1 => congr_Sort (eq_refl s0) (eq_refl s1)
-  | Pi s0 s1 s2 s3 =>
-      congr_Pi (eq_refl s0) (eq_refl s1)
-        (extRen_term xi_term zeta_term Eq_term s2)
+  | Pi s0 s1 s2 s3 s4 s5 =>
+      congr_Pi (eq_refl s0) (eq_refl s1) (eq_refl s2) (eq_refl s3)
+        (extRen_term xi_term zeta_term Eq_term s4)
         (extRen_term (upRen_term_term xi_term) (upRen_term_term zeta_term)
-           (upExtRen_term_term _ _ Eq_term) s3)
+           (upExtRen_term_term _ _ Eq_term) s5)
   | lam s0 s1 s2 =>
       congr_lam (eq_refl s0) (extRen_term xi_term zeta_term Eq_term s1)
         (extRen_term (upRen_term_term xi_term) (upRen_term_term zeta_term)
@@ -316,11 +324,11 @@ subst_term sigma_term s = subst_term tau_term s :=
   match s with
   | var s0 => Eq_term s0
   | Sort s0 s1 => congr_Sort (eq_refl s0) (eq_refl s1)
-  | Pi s0 s1 s2 s3 =>
-      congr_Pi (eq_refl s0) (eq_refl s1)
-        (ext_term sigma_term tau_term Eq_term s2)
+  | Pi s0 s1 s2 s3 s4 s5 =>
+      congr_Pi (eq_refl s0) (eq_refl s1) (eq_refl s2) (eq_refl s3)
+        (ext_term sigma_term tau_term Eq_term s4)
         (ext_term (up_term_term sigma_term) (up_term_term tau_term)
-           (upExt_term_term _ _ Eq_term) s3)
+           (upExt_term_term _ _ Eq_term) s5)
   | lam s0 s1 s2 =>
       congr_lam (eq_refl s0) (ext_term sigma_term tau_term Eq_term s1)
         (ext_term (up_term_term sigma_term) (up_term_term tau_term)
@@ -370,12 +378,12 @@ Fixpoint compRenRen_term (xi_term : nat -> nat) (zeta_term : nat -> nat)
   match s with
   | var s0 => ap (var) (Eq_term s0)
   | Sort s0 s1 => congr_Sort (eq_refl s0) (eq_refl s1)
-  | Pi s0 s1 s2 s3 =>
-      congr_Pi (eq_refl s0) (eq_refl s1)
-        (compRenRen_term xi_term zeta_term rho_term Eq_term s2)
+  | Pi s0 s1 s2 s3 s4 s5 =>
+      congr_Pi (eq_refl s0) (eq_refl s1) (eq_refl s2) (eq_refl s3)
+        (compRenRen_term xi_term zeta_term rho_term Eq_term s4)
         (compRenRen_term (upRen_term_term xi_term)
            (upRen_term_term zeta_term) (upRen_term_term rho_term)
-           (up_ren_ren _ _ _ Eq_term) s3)
+           (up_ren_ren _ _ _ Eq_term) s5)
   | lam s0 s1 s2 =>
       congr_lam (eq_refl s0)
         (compRenRen_term xi_term zeta_term rho_term Eq_term s1)
@@ -434,12 +442,12 @@ subst_term tau_term (ren_term xi_term s) = subst_term theta_term s :=
   match s with
   | var s0 => Eq_term s0
   | Sort s0 s1 => congr_Sort (eq_refl s0) (eq_refl s1)
-  | Pi s0 s1 s2 s3 =>
-      congr_Pi (eq_refl s0) (eq_refl s1)
-        (compRenSubst_term xi_term tau_term theta_term Eq_term s2)
+  | Pi s0 s1 s2 s3 s4 s5 =>
+      congr_Pi (eq_refl s0) (eq_refl s1) (eq_refl s2) (eq_refl s3)
+        (compRenSubst_term xi_term tau_term theta_term Eq_term s4)
         (compRenSubst_term (upRen_term_term xi_term) (up_term_term tau_term)
            (up_term_term theta_term) (up_ren_subst_term_term _ _ _ Eq_term)
-           s3)
+           s5)
   | lam s0 s1 s2 =>
       congr_lam (eq_refl s0)
         (compRenSubst_term xi_term tau_term theta_term Eq_term s1)
@@ -509,12 +517,12 @@ ren_term zeta_term (subst_term sigma_term s) = subst_term theta_term s :=
   match s with
   | var s0 => Eq_term s0
   | Sort s0 s1 => congr_Sort (eq_refl s0) (eq_refl s1)
-  | Pi s0 s1 s2 s3 =>
-      congr_Pi (eq_refl s0) (eq_refl s1)
-        (compSubstRen_term sigma_term zeta_term theta_term Eq_term s2)
+  | Pi s0 s1 s2 s3 s4 s5 =>
+      congr_Pi (eq_refl s0) (eq_refl s1) (eq_refl s2) (eq_refl s3)
+        (compSubstRen_term sigma_term zeta_term theta_term Eq_term s4)
         (compSubstRen_term (up_term_term sigma_term)
            (upRen_term_term zeta_term) (up_term_term theta_term)
-           (up_subst_ren_term_term _ _ _ Eq_term) s3)
+           (up_subst_ren_term_term _ _ _ Eq_term) s5)
   | lam s0 s1 s2 =>
       congr_lam (eq_refl s0)
         (compSubstRen_term sigma_term zeta_term theta_term Eq_term s1)
@@ -593,12 +601,12 @@ subst_term tau_term (subst_term sigma_term s) = subst_term theta_term s :=
   match s with
   | var s0 => Eq_term s0
   | Sort s0 s1 => congr_Sort (eq_refl s0) (eq_refl s1)
-  | Pi s0 s1 s2 s3 =>
-      congr_Pi (eq_refl s0) (eq_refl s1)
-        (compSubstSubst_term sigma_term tau_term theta_term Eq_term s2)
+  | Pi s0 s1 s2 s3 s4 s5 =>
+      congr_Pi (eq_refl s0) (eq_refl s1) (eq_refl s2) (eq_refl s3)
+        (compSubstSubst_term sigma_term tau_term theta_term Eq_term s4)
         (compSubstSubst_term (up_term_term sigma_term)
            (up_term_term tau_term) (up_term_term theta_term)
-           (up_subst_subst_term_term _ _ _ Eq_term) s3)
+           (up_subst_subst_term_term _ _ _ Eq_term) s5)
   | lam s0 s1 s2 =>
       congr_lam (eq_refl s0)
         (compSubstSubst_term sigma_term tau_term theta_term Eq_term s1)
@@ -729,11 +737,11 @@ Fixpoint rinst_inst_term (xi_term : nat -> nat) (sigma_term : nat -> term)
   match s with
   | var s0 => Eq_term s0
   | Sort s0 s1 => congr_Sort (eq_refl s0) (eq_refl s1)
-  | Pi s0 s1 s2 s3 =>
-      congr_Pi (eq_refl s0) (eq_refl s1)
-        (rinst_inst_term xi_term sigma_term Eq_term s2)
+  | Pi s0 s1 s2 s3 s4 s5 =>
+      congr_Pi (eq_refl s0) (eq_refl s1) (eq_refl s2) (eq_refl s3)
+        (rinst_inst_term xi_term sigma_term Eq_term s4)
         (rinst_inst_term (upRen_term_term xi_term) (up_term_term sigma_term)
-           (rinstInst_up_term_term _ _ Eq_term) s3)
+           (rinstInst_up_term_term _ _ Eq_term) s5)
   | lam s0 s1 s2 =>
       congr_lam (eq_refl s0) (rinst_inst_term xi_term sigma_term Eq_term s1)
         (rinst_inst_term (upRen_term_term xi_term) (up_term_term sigma_term)
@@ -965,11 +973,13 @@ Fixpoint allfv_term (p_term : nat -> Prop) (s : term) {struct s} : Prop :=
   match s with
   | var s0 => p_term s0
   | Sort s0 s1 => and True (and True True)
-  | Pi s0 s1 s2 s3 =>
+  | Pi s0 s1 s2 s3 s4 s5 =>
       and True
         (and True
-           (and (allfv_term p_term s2)
-              (and (allfv_term (upAllfv_term_term p_term) s3) True)))
+           (and True
+              (and True
+                 (and (allfv_term p_term s4)
+                    (and (allfv_term (upAllfv_term_term p_term) s5) True)))))
   | lam s0 s1 s2 =>
       and True
         (and (allfv_term p_term s1)
@@ -1009,13 +1019,15 @@ Fixpoint allfvTriv_term (p_term : nat -> Prop) (H_term : forall x, p_term x)
   match s with
   | var s0 => H_term s0
   | Sort s0 s1 => conj I (conj I I)
-  | Pi s0 s1 s2 s3 =>
+  | Pi s0 s1 s2 s3 s4 s5 =>
       conj I
         (conj I
-           (conj (allfvTriv_term p_term H_term s2)
-              (conj
-                 (allfvTriv_term (upAllfv_term_term p_term)
-                    (upAllfvTriv_term_term H_term) s3) I)))
+           (conj I
+              (conj I
+                 (conj (allfvTriv_term p_term H_term s4)
+                    (conj
+                       (allfvTriv_term (upAllfv_term_term p_term)
+                          (upAllfvTriv_term_term H_term) s5) I)))))
   | lam s0 s1 s2 =>
       conj I
         (conj (allfvTriv_term p_term H_term s1)
@@ -1068,36 +1080,51 @@ allfv_term p_term s -> allfv_term q_term s :=
   match s with
   | var s0 => fun HP => H_term s0 HP
   | Sort s0 s1 => fun HP => conj I (conj I I)
-  | Pi s0 s1 s2 s3 =>
+  | Pi s0 s1 s2 s3 s4 s5 =>
       fun HP =>
       conj I
         (conj I
-           (conj
-              (allfvImpl_term p_term q_term H_term s2
-                 match HP with
-                 | conj _ HP =>
-                     match HP with
-                     | conj _ HP => match HP with
-                                    | conj HP _ => HP
-                                    end
-                     end
-                 end)
-              (conj
-                 (allfvImpl_term (upAllfv_term_term p_term)
-                    (upAllfv_term_term q_term) (upAllfvImpl_term_term H_term)
-                    s3
-                    match HP with
-                    | conj _ HP =>
-                        match HP with
-                        | conj _ HP =>
-                            match HP with
-                            | conj _ HP =>
-                                match HP with
-                                | conj HP _ => HP
-                                end
-                            end
-                        end
-                    end) I)))
+           (conj I
+              (conj I
+                 (conj
+                    (allfvImpl_term p_term q_term H_term s4
+                       match HP with
+                       | conj _ HP =>
+                           match HP with
+                           | conj _ HP =>
+                               match HP with
+                               | conj _ HP =>
+                                   match HP with
+                                   | conj _ HP =>
+                                       match HP with
+                                       | conj HP _ => HP
+                                       end
+                                   end
+                               end
+                           end
+                       end)
+                    (conj
+                       (allfvImpl_term (upAllfv_term_term p_term)
+                          (upAllfv_term_term q_term)
+                          (upAllfvImpl_term_term H_term) s5
+                          match HP with
+                          | conj _ HP =>
+                              match HP with
+                              | conj _ HP =>
+                                  match HP with
+                                  | conj _ HP =>
+                                      match HP with
+                                      | conj _ HP =>
+                                          match HP with
+                                          | conj _ HP =>
+                                              match HP with
+                                              | conj HP _ => HP
+                                              end
+                                          end
+                                      end
+                                  end
+                              end
+                          end) I)))))
   | lam s0 s1 s2 =>
       fun HP =>
       conj I
@@ -1288,36 +1315,52 @@ allfv_term (funcomp p_term xi_term) s :=
   match s with
   | var s0 => fun H => H
   | Sort s0 s1 => fun H => conj I (conj I I)
-  | Pi s0 s1 s2 s3 =>
+  | Pi s0 s1 s2 s3 s4 s5 =>
       fun H =>
       conj I
         (conj I
-           (conj
-              (allfvRenL_term p_term xi_term s2
-                 match H with
-                 | conj _ H =>
-                     match H with
-                     | conj _ H => match H with
-                                   | conj H _ => H
-                                   end
-                     end
-                 end)
-              (conj
-                 (allfvImpl_term _ _ (upAllfvRenL_term_term p_term xi_term)
-                    s3
-                    (allfvRenL_term (upAllfv_term_term p_term)
-                       (upRen_term_term xi_term) s3
+           (conj I
+              (conj I
+                 (conj
+                    (allfvRenL_term p_term xi_term s4
                        match H with
                        | conj _ H =>
                            match H with
                            | conj _ H =>
                                match H with
-                               | conj _ H => match H with
-                                             | conj H _ => H
-                                             end
+                               | conj _ H =>
+                                   match H with
+                                   | conj _ H =>
+                                       match H with
+                                       | conj H _ => H
+                                       end
+                                   end
                                end
                            end
-                       end)) I)))
+                       end)
+                    (conj
+                       (allfvImpl_term _ _
+                          (upAllfvRenL_term_term p_term xi_term) s5
+                          (allfvRenL_term (upAllfv_term_term p_term)
+                             (upRen_term_term xi_term) s5
+                             match H with
+                             | conj _ H =>
+                                 match H with
+                                 | conj _ H =>
+                                     match H with
+                                     | conj _ H =>
+                                         match H with
+                                         | conj _ H =>
+                                             match H with
+                                             | conj _ H =>
+                                                 match H with
+                                                 | conj H _ => H
+                                                 end
+                                             end
+                                         end
+                                     end
+                                 end
+                             end)) I)))))
   | lam s0 s1 s2 =>
       fun H =>
       conj I
@@ -1501,36 +1544,52 @@ allfv_term p_term (ren_term xi_term s) :=
   match s with
   | var s0 => fun H => H
   | Sort s0 s1 => fun H => conj I (conj I I)
-  | Pi s0 s1 s2 s3 =>
+  | Pi s0 s1 s2 s3 s4 s5 =>
       fun H =>
       conj I
         (conj I
-           (conj
-              (allfvRenR_term p_term xi_term s2
-                 match H with
-                 | conj _ H =>
-                     match H with
-                     | conj _ H => match H with
-                                   | conj H _ => H
-                                   end
-                     end
-                 end)
-              (conj
-                 (allfvRenR_term (upAllfv_term_term p_term)
-                    (upRen_term_term xi_term) s3
-                    (allfvImpl_term _ _
-                       (upAllfvRenR_term_term p_term xi_term) s3
+           (conj I
+              (conj I
+                 (conj
+                    (allfvRenR_term p_term xi_term s4
                        match H with
                        | conj _ H =>
                            match H with
                            | conj _ H =>
                                match H with
-                               | conj _ H => match H with
-                                             | conj H _ => H
-                                             end
+                               | conj _ H =>
+                                   match H with
+                                   | conj _ H =>
+                                       match H with
+                                       | conj H _ => H
+                                       end
+                                   end
                                end
                            end
-                       end)) I)))
+                       end)
+                    (conj
+                       (allfvRenR_term (upAllfv_term_term p_term)
+                          (upRen_term_term xi_term) s5
+                          (allfvImpl_term _ _
+                             (upAllfvRenR_term_term p_term xi_term) s5
+                             match H with
+                             | conj _ H =>
+                                 match H with
+                                 | conj _ H =>
+                                     match H with
+                                     | conj _ H =>
+                                         match H with
+                                         | conj _ H =>
+                                             match H with
+                                             | conj _ H =>
+                                                 match H with
+                                                 | conj H _ => H
+                                                 end
+                                             end
+                                         end
+                                     end
+                                 end
+                             end)) I)))))
   | lam s0 s1 s2 =>
       fun H =>
       conj I
