theories/BasicMetaTheory.v
@@ -282,13 +282,13 @@ Proof.
 Qed.
 
 Lemma scope_pi_inv :
-  ∀ Γ mx m A B m',
-    scoping Γ (Pi m mx A B) m' →
+  ∀ Γ i j mx m A B m',
+    scoping Γ (Pi i j m mx A B) m' →
     scoping Γ A mKind ∧
     scoping (mx :: Γ) B mKind ∧
     m' = mKind.
 Proof.
-  intros Γ mx m A B m' h.
+  intros Γ i j mx m A B m' h.
   inversion h. subst.
   intuition eauto.
 Qed.
@@ -758,19 +758,18 @@ Proof.
 Qed.
 
 Lemma type_pi_inv :
-  ∀ Γ mx m A B C,
-    Γ ⊢ Pi m mx A B : C →
-    ∃ i j,
-      cscoping Γ A mKind ∧
-      cscoping (Γ ,, (mx, A)) B mKind ∧
-      Γ ⊢ A : Sort mx i ∧
-      Γ ,, (mx, A) ⊢ B : Sort m j ∧
-      Γ ⊢ Sort m (max i j) ≡ C.
+  ∀ Γ i j mx m A B C,
+    Γ ⊢ Pi i j m mx A B : C →
+    cscoping Γ A mKind ∧
+    cscoping (Γ ,, (mx, A)) B mKind ∧
+    Γ ⊢ A : Sort mx i ∧
+    Γ ,, (mx, A) ⊢ B : Sort m j ∧
+    Γ ⊢ Sort m (max i j) ≡ C.
 Proof.
-  intros ?????? h.
+  intros ???????? h.
   dependent induction h.
-  - eexists _,_. intuition eauto. constructor.
-  - destruct_exists IHh1. eexists _,_. intuition eauto.
+  - intuition eauto. constructor.
+  - intuition eauto.
     eapply conv_trans. all: eauto.
 Qed.
 
@@ -780,7 +779,7 @@ Ltac ttinv h h' :=
     lazymatch t with
     | var _ => eapply type_var_inv in h as h'
     | Sort _ _ => eapply type_sort_inv in h as h'
-    | Pi _ _ _ _ => eapply type_pi_inv in h as h'
+    | Pi _ _ _ _ _ _ => eapply type_pi_inv in h as h'
     end
   end.
 
@@ -800,7 +799,7 @@ Ltac unitac h1 h2 :=
 
 Derive Signature for conversion.
 
-Lemma conv_sort_inv :
+(* Lemma conv_sort_inv :
   ∀ Γ m i j,
     Γ ⊢ Sort m i ≡ Sort m j →
     m = mProp ∨ i = j.
@@ -810,7 +809,7 @@ Proof.
   - (* We're not going to be able to prove it this way. *)
     admit.
   - inversion H.
-Abort.
+Abort. *)
 
 Lemma type_unique :
   ∀ Γ t A B,
@@ -823,16 +822,5 @@ Proof.
   all: try unitac hA hB. all: try assumption.
   - eapply meta_conv_trans_l. 2: eassumption.
     f_equal. congruence.
-  - eapply conv_trans. 2: eassumption.
-    eapply IHt1 in H2. 2: eassumption.
-    eapply IHt2 in H5. 2: eassumption.
-    (* Without conv_sort_inv we can only hope for uniqueness modulo
-      universe levels. Maybe it's a good idea to generalise already to
-      principal typing?
-      I don't really need conversion for the proof.
-
-      It might be a good idea to progress with the rest instead, as we might
-      later have more power to prove this lemma, and it won't be needed for
-      a while.
-     *)
+  -
 Abort.
