theories/TermMode.v
@@ -20,7 +20,7 @@ Section Mode.
     match t with
     | var x => nth x Γ dummy
     | Sort m l => mKind
-    | Pi m mx A B => mKind
+    | Pi i j m mx A B => mKind
     | lam mx A t => md (mx :: Γ) t
     | app u v => md Γ u
     | Erased A => mKind
